Logic/Modal/Normal/HilbertStyle.lean
@@ -89,7 +89,7 @@ variable {α : Type u}
 /--
   Hilbert-style deduction system
 -/
-inductive Deduction (Λ : Logic (Formula α)) : Set (Formula α) → (Formula α) → Type _
+inductive Deduction (Λ : Logic α) : Set (Formula α) → (Formula α) → Type _
   | axm {Γ p}            : p ∈ Γ → Deduction Λ Γ p
   | maxm {Γ p}           : p ∈ Λ → Deduction Λ Γ p
   | modus_ponens {Γ p q} : Deduction Λ Γ (p ⟶ q) → Deduction Λ Γ p → Deduction Λ Γ q
@@ -108,7 +108,7 @@ inductive Deduction (Λ : Logic (Formula α)) : Set (Formula α) → (Formula α
 
 notation:45 Γ " ⊢ᴹ(" Λ ") " p => Deduction Λ Γ p
 
-variable (Λ : Logic (Formula α)) (Γ : Set (Formula α)) (p : Formula α)
+variable (Λ : Logic α) (Γ : Set (Formula α)) (p : Formula α)
 
 abbrev Deducible := Nonempty (Γ ⊢ᴹ(Λ) p)
 notation:45 Γ " ⊢ᴹ(" Λ ")! " p => Deducible Λ Γ p
@@ -174,7 +174,7 @@ def length {Γ : Set (Formula α)} {p : Formula α} : (Γ ⊢ᴹ(Λ) p) → ℕ
   | necessitation d₁ => d₁.length + 1
   | _ => 0
 
-variable {Λ : Logic (Formula α)} {Γ : Set (Formula α)} {p q : Formula α}
+variable {Λ : Logic α} {Γ : Set (Formula α)} {p q : Formula α}
 
 protected def cast (d : Γ ⊢ᴹ(Λ) p) (e₁ : Γ = Δ) (e₂ : p = q) : Δ ⊢ᴹ(Λ) q := cast (by simp [e₁,e₂]) d
 
