README.md
@@ -148,9 +148,9 @@ In this formalization, _(Modal) Logic_ means set of axioms.
   theorem LO.Modal.Normal.Logic.Hilbert.sounds
       {α : Type u}
       {β : Type u} [Inhabited β]
-      (Λ : Logic (Formula α)) [LogicDefines α β Λ]
+      (Λ : Logic α)
+      (f : Frame β) (hf : f ∈ (FrameClass β α Λ))
       {p : LO.Modal.Normal.Formula α}
-      (f : LO.Modal.Normal.Frame β) (hf : LogicDefines.definability Λ f.rel)
       (h : ⊢ᴹ(Λ) p) :
       ⊧ᴹᶠ[f] p
   ```
@@ -159,7 +159,8 @@ In this formalization, _(Modal) Logic_ means set of axioms.
     theorem LO.Modal.Normal.Logic.Hilbert.consistency
         {α : Type u}
         {β : Type u}
-        (Λ : Logic (Formula α)) [LogicDefines α β Λ] :
+        (Λ : Logic α)
+        (hf : ∃ f, f ∈ (FrameClass β α Λ)) :
         ⊬ᴹ(Λ)! ⊥
     ```
   -  **WIP:** Currently, these theorems was proved where only `Λ` is `𝐊`, `𝐊𝐃`. For example, if it is proved that `𝐒𝟒` defines some frame reachability (i.e. satisfies `LogicDefines`), then these theorems are obviously proved.
